

LTI MPC

$$x(t) = \begin{bmatrix} \text{soc}(t) \\ E_{\text{fuel}}(t) \end{bmatrix}$$

$\xrightarrow{e[P]}$
 $\xrightarrow{[J]}$

$$u(t) = \begin{bmatrix} P_e(t) \\ P_m(t) \end{bmatrix}$$

Disturbance $\rightarrow P_{\text{dem}}(t) = P_{\text{sh-req}}(t)$

(constants) $\rightarrow E_{\text{batt,nom}} = V_{\text{nom}} Q_{\text{Ah}} \cdot 3600 [\text{J}]$

$$\boxed{\eta_e = 0.22 \quad \eta_m = 0.75}$$

Differential Eq^s

Battery DE :

$$P_{\text{cell,m}}(t) = \frac{P_m(t)}{\eta_m \times \eta_{\text{batt}}}$$

$$E_{\text{batt}}(t) = \text{soc}(t) \times E_{\text{batt,nom}}$$

$$\frac{dE_{\text{batt}}(t)}{dt} = -P_{\text{cell,m}}(t) \Rightarrow E_{\text{batt,nom}} \frac{d(\text{soc}(t))}{dt} = -\frac{P_m(t)}{\eta_m \times \eta_{\text{batt}}}$$

$$\dot{\text{soc}}(t) = -\frac{1}{E_{\text{batt,nom}} \times \eta_m \times \eta_{\text{batt}}} \times P_m(t)$$

Fuel DE :

$$P_{\text{fuel,in}}(t) = \frac{P_e(t)}{\eta_e}$$

~~Assuming fuel conversion efficiency~~
Assuming fuel conversion efficiency + engine efficiency is lumped!

$$\frac{dE_{\text{fuel}}}{dt} = -P_{\text{fuel,in}}(t) = -\frac{P_e(t)}{\eta_e}$$

$$\dot{E}_{\text{fuel}} = -\frac{1}{\eta_e} \times P_e(t)$$

Vector form / Matrix form

$$\dot{x}(t) = \begin{bmatrix} \dot{soc}(t) \\ \dot{E}_{fuel}(t) \end{bmatrix}$$

$$x(t) = \begin{bmatrix} soc(t) \\ E_{fuel}(t) \end{bmatrix}$$

$$u(t) = \begin{bmatrix} P_e(t) \\ P_m(t) \end{bmatrix}$$

$$\dot{soc} = -\frac{1}{E_{battery} \eta_b} P_e(t)$$

$$\dot{E}_{fuel} = -\frac{1}{\eta_b} x P_e(t)$$

$$\dot{x}(t) = A x(t) + B u(t)$$

$$y(t) = C x(t) + D u(t)$$

$$A = \begin{bmatrix} 0 & 0 \\ 0 & 0 \end{bmatrix}$$

$$B = \begin{bmatrix} 0 & -\frac{1}{E_{battery} \eta_b} \\ \frac{1}{\eta_b} & 0 \end{bmatrix}$$

$$C = \begin{bmatrix} 1 & 0 \\ 0 & 1 \end{bmatrix}$$

$$D = \begin{bmatrix} 0 & 0 \\ 0 & 0 \end{bmatrix}$$

$$\dot{x}(t) = A x(t) + B u(t)$$

$$\frac{x_{k+1} - x_k}{T_s} = A x_k + B u_k \Rightarrow x_{k+1} = x_k + T_s A x_k + T_s B u_k$$

$$x_{k+1} = (I_2 + T_s A) x_k + T_s B u_k$$

$$x_{k+1} = A_d x_k + B_d u_k$$

$$A_d = \begin{bmatrix} 1 & 0 \\ 0 & 1 \end{bmatrix}$$

$$B_d = \begin{bmatrix} 0 & -T_s \\ \frac{T_s}{\eta_b} & 0 \end{bmatrix}$$

$$y_k = C_d x_k + D u_k$$

$$C_d = \begin{bmatrix} 1 & 0 \\ 0 & 1 \end{bmatrix}$$

$$D = \begin{bmatrix} 0 & 0 \\ 0 & 0 \end{bmatrix}$$

Cost function

$$Q = \begin{bmatrix} q_{soc} & 0 \\ 0 & q_{fuel} \end{bmatrix}$$

$$R = \begin{bmatrix} r_e & 0 \\ 0 & r_m \end{bmatrix}$$

$$S = \begin{bmatrix} s_{soc} & 0 \\ 0 & s_{fuel} \end{bmatrix}$$

$$L(k) = \underbrace{(y(k) - y_{ref}(k))^T Q (y(k) - y_{ref}(k))}_{\text{Error}} + \underbrace{u(k)^T R u(k)}_{\text{input wt.}}$$

predicted horizon

Prediction Step

$$h = N_p$$

$$X = \begin{bmatrix} x(k+1) \\ x(k+2) \\ \vdots \\ x(k+h) \end{bmatrix}$$

$$U = \begin{bmatrix} u(k) \\ u(k+1) \\ \vdots \\ u(k+h-1) \end{bmatrix}$$

$$x_{k+1} = A_d x(k) + B_d u(k)$$

$$x_{k+2} = A_d (A_d x(k) + B_d u(k)) + B_d u(k+1)$$

$$x_{k+2} = A_d^2 x(k) + A_d B_d u(k) + B_d u(k+1)$$

$$x_{k+i} = A_d^i x(k) + \sum_{j=0}^{i-1} A_d^{i-j-1} B_d u(k+j)$$

$$\begin{bmatrix} x_{k+1} \\ x_{k+2} \\ \vdots \\ x_{k+h} \end{bmatrix} = \begin{bmatrix} A_d \\ A_d^2 \\ \vdots \\ A_d^h \end{bmatrix} x(k) + \begin{bmatrix} B_d & A_d B_d & \dots & A_d^{h-1} B_d \end{bmatrix} \begin{bmatrix} u(k) \\ u(k+1) \\ \vdots \\ u(k+h-1) \end{bmatrix}$$

$$X = \begin{bmatrix} A_d & B_d \\ A_d^2 & A_d B_d & B_d \\ \vdots & \vdots & \vdots \\ A_d^h & A_d^{h-1} B_d & \dots & B_d \end{bmatrix} \begin{bmatrix} x(k) \\ u(k) \\ \vdots \\ u(k+h-1) \end{bmatrix}$$

predicted

initial

$$\begin{aligned} y_{k+1} &= C_d x_{k+1} \\ y_{k+2} &= C_d x_{k+2} \\ &\vdots \\ y_{k+N} &= C_d x_{k+N} \end{aligned}$$

$$\begin{bmatrix} y_{k+1} \\ y_{k+2} \\ \vdots \\ y_{k+N} \end{bmatrix}_{2h \times 1} = \begin{bmatrix} C_d A^1 & C_d A^2 & \dots & C_d A^N \\ C_d A^2 & C_d A^3 & \dots & C_d A^{N+1} \\ \vdots & \vdots & \ddots & \vdots \\ C_d A^N & C_d A^{N+1} & \dots & C_d A^{N+N} \end{bmatrix}_{2h \times 2h} \begin{bmatrix} x_{k+1} \\ x_{k+2} \\ x_{k+3} \\ \vdots \\ x_{k+N} \end{bmatrix}_{2h \times 1}$$

$$y_{ref, h} = \begin{bmatrix} soc(x_k) \\ E_{fuel}(k) \end{bmatrix} = \begin{bmatrix} 0.6 \\ E_{fuel}(k) \end{bmatrix}$$

$$soc(x) < 0.25 \rightarrow u$$



$$y = C_H x + D_H u$$

$$D_H = 0$$

$$y_{ref, h} = \begin{bmatrix} y_{ref}(k+1) \\ y_{ref}(k+2) \\ \vdots \\ y_{ref}(k+h) \end{bmatrix}$$

$$Q_H = \begin{bmatrix} Q & & & \\ & Q & & \\ & & \ddots & \\ & & & Q \end{bmatrix}_{2h \times 2h}$$

$$R_H = \begin{bmatrix} R & & \\ & R & \\ & & \ddots \\ & & & R \end{bmatrix}_{2h \times 2h}$$

$$J = (y - y_{ref, h})^T_{1 \times 2h} Q_H (y - y_{ref, h})_{2h \times 1} + U^T_{2h \times 1} R_H U_{2h \times 1}$$

$$x = A_H x_k + B_H u$$

$$y = C_H x + D_H u$$

$$y = C_H A_H x_k + C_H B_H u$$

$$J = (y - y_{ref, h})^T Q_H (y - y_{ref, h}) + U^T R_H U$$

$$J = (C_H A_H x_k - y_{ref, h})^T Q_H (C_H A_H x_k - y_{ref, h}) + U^T R_H U$$

$$\text{Substitute } x = A_H x_k + B_H u$$

$$J =$$

$$J = (Y - Y_{ref,h})^T Q_H (Y - Y_{ref,h}) + U^T R_H U$$

$$J = (C_H A_H x_k + C_H B_H U - Y_{ref,h})^T Q_H (C_H A_H x_k + C_H B_H U - Y_{ref,h}) + U^T R_H U$$

$$J = (x_k^T A_H^T C_H^T + U^T B_H^T C_H^T - Y_{ref,h}^T) Q_H (C_H A_H x_k + C_H B_H U - Y_{ref,h}) + U^T R_H U$$

Assuming $E = C_H A_H x_k - Y_{ref,h}$ & $C_H B_H = G$
 Substituting E in above eqn: Constant for one gain of controller

$$J = (E^T - U^T G^T) Q_H (E - G U) + U^T R_H U$$

$$J = E^T Q_H E - E^T Q_H G U - U^T G^T Q_H E + U^T G^T Q_H G U + U^T R_H U$$

$$J = E^T Q_H E - E^T Q_H G U - U^T (G^T Q_H E +$$

$$J = E^T Q_H E - E^T Q_H G U - U^T G^T Q_H E + U^T (G^T Q_H G + R_H) U$$

As Q_H is a symmetric matrix, $Q_H = Q_H^T$

$$J = E^T Q_H E - E^T Q_H G U - U^T G^T Q_H E + U^T (G^T Q_H G + R_H) U$$

$$J = E^T Q_H E - E^T Q_H G U - (E^T Q_H G U)^T + U^T (G^T Q_H G + R_H) U$$

As both are scalars then we can omit transpose as the values after solving them will be one dimensional (1x1).

$$J = \underbrace{E^T Q_H E}_{\text{Constant}} - \underbrace{2 E^T Q_H G U}_{2(U^T G^T Q_H E) \text{ linear or}} + \underbrace{U^T (G^T Q_H G + R_H) U}_{\text{Quadratic}}$$

Substituting all values we found:

$$J = (C_H A_H x_k - Y_{ref,h})^T Q_H (C_H A_H x_k - Y_{ref,h}) - 2 (C_H A_H x_k - Y_{ref,h})^T Q_H C_H B_H U + U^T (C_H B_H)^T Q_H (C_H B_H) + R_H) U$$

$$J = a_0 + a_1 U + a_2 U^T$$

$$J = \frac{1}{2} a_0 + \frac{1}{2} a_1 U + \frac{1}{2} U^T a_2 U$$

Divide by 2

$$\frac{\partial J}{\partial U} = \frac{1}{2} a_1 + \frac{1}{2} a_2 U = 0 \quad \left\{ \frac{\partial (a_0/2)}{\partial U} = 0 \right\}$$

$$a_2 U^* = -\frac{1}{2} a_1$$

$$U^* = -\frac{1}{2} \frac{a_1}{a_2}$$

We can remove $\frac{a_0}{2}$ from cost function as it is just increasing computational time and processing power.

$$J^* = \frac{1}{2} a_2^{-1} a_1$$

$$\begin{cases} a_1 = -2(C_H A_H x_k - y_{ref,h}) \cdot Q_H \cdot C_H B_H \\ a_2 = (C_H B_H)^T \cdot Q_H \cdot C_H B_H + R_H \end{cases}$$

$$J^* = \frac{1}{2} (-2) \times [(C_H A_H x_k - y_{ref,h}) \cdot Q_H \cdot C_H B_H] \cdot [(C_H B_H)^T \cdot Q_H \cdot C_H B_H + R_H]$$

$$U^* = (C_H A_H x_k - y_{ref,h}) \cdot Q_H \cdot C_H B_H \cdot [(C_H B_H)^T \cdot Q_H \cdot C_H B_H + R_H]^{-1}$$

$$[C_H]_{2N \times 2N} = \begin{bmatrix} I_2 & & \\ & I_2 & \\ & & \ddots \\ & & & I_2 \end{bmatrix}_{2N \times 2N}$$

$$B_H = \begin{bmatrix} B_d & & \\ & B_d & \\ & & \ddots \\ & & & B_d \end{bmatrix}_{2N \times 2N}$$

$$A_H = \begin{bmatrix} A_d & \\ & A_d \\ & \ddots \\ & & A_d \end{bmatrix}_{2N \times 2N} \rightarrow \begin{bmatrix} 1 & 0 \\ 0 & 1 \end{bmatrix}_{2 \times 2}$$

$$U^* = \begin{bmatrix} u_{k+1}^* \\ \vdots \\ u_{k+N-1}^* \end{bmatrix}_{2N \times 1}$$

Input $\leftarrow u_k = \begin{bmatrix} p_{e,k} \\ p_{m,k} \end{bmatrix}_{2 \times 1}$

$$x_k = \begin{bmatrix} \omega_{soc,k} \\ E_{fuel,k} \end{bmatrix}_{2 \times 1}$$

$$y_{ref,h} = \begin{bmatrix} y_{ref,k+1} \\ y_{ref,k+2} \\ \vdots \\ y_{ref,k+N} \end{bmatrix}_{2N \times 1}$$

$$R_H = \begin{bmatrix} R & & \\ & R & \\ & & \ddots \\ & & & R \end{bmatrix}_{2N \times 2N}$$

$$Q_H = \begin{bmatrix} Q & & \\ & Q & \\ & & \ddots \\ & & & Q \end{bmatrix}_{2N \times 2N}$$

$$U^* = [(C_H A_H x_k - y_{ref,h}) \cdot Q_H \cdot C_H B_H] \cdot [(C_H B_H)^T \cdot Q_H \cdot C_H B_H + R_H]^{-1}$$

$$U^* = \begin{bmatrix} Q_H \cdot C_H B_H \cdot (C_H A_H x_k - y_{ref,h}) \\ \vdots \\ Q_H \cdot C_H B_H \cdot (C_H A_H x_k - y_{ref,h}) \end{bmatrix} \cdot [(C_H B_H)^T \cdot Q_H \cdot C_H B_H + R_H]^{-1}$$

$$U^* = -\frac{1}{2} E a_2^{-1} a_1 \rightarrow \begin{cases} a_1 = -2(C_H A_H x_k - y_{ref,h}) \cdot Q_H \cdot C_H \cdot B_H \\ a_2 = (C_H B_H)^T \cdot Q_H \cdot (C_H \cdot B_H) + R_H \end{cases}$$

$$U^* = -\frac{1}{2} \times (-2) \cdot \left[(C_H B_H)^T \cdot Q_H \cdot (C_H \cdot B_H) + R_H \right]^{-1} \cdot \begin{bmatrix} (C_H A_H x_k - y_{ref,h}) \cdot Q_H \cdot C_H \cdot B_H \\ Q_H \cdot C_H \cdot B_H \end{bmatrix}$$

$$U^* = \left[(C_H B_H)^T \cdot Q_H \cdot (C_H \cdot B_H) + R_H \right]^{-1} \cdot \left[(C_H A_H x_k - y_{ref,h}) \cdot Q_H \cdot C_H \cdot B_H \right]$$

$$\left(\underbrace{(C_H B_H)^T}_{2N \times 2N} \cdot \underbrace{Q_H}_{2N \times 2N} \cdot \underbrace{(C_H \cdot B_H)}_{2N \times 2N} + \underbrace{R_H}_{2N \times 2N} \right)^{-1} = \boxed{2N \times 2N}$$

$$\underbrace{(C_H A_H x_k - y_{ref,h})^T}_{2N \times 2N} \cdot \underbrace{Q_H}_{2N \times 2N} \cdot \underbrace{C_H \cdot B_H}_{2 \times 1} \rightarrow \begin{matrix} 2N \times 1 & 2N \times 1 \\ \hline 2N \times 1 \end{matrix} \quad \underbrace{2N \times 2N}$$

$$f^T = [E^T \cdot Q_H \cdot G]$$

If I used $\frac{1}{2} U^T G^T Q_H G U + \frac{1}{2} U^T (G^T Q_H G + R_H) U$

$$\frac{\partial J}{\partial U} = \underbrace{-G^T Q_H E}_{f^T} + \underbrace{(G^T Q_H G + R_H)}_{H} \cdot U$$

constant linear quadratic

$$as f = [E^T Q_H G] \quad H = G^T Q_H G + R_H$$

$$\boxed{f = (C_H A_H x_k - y_{ref,h})^T \cdot Q_H \cdot (C_H \cdot B_H)} \quad \boxed{H = (C_H B_H)^T \cdot Q_H \cdot (C_H \cdot B_H) + R_H}$$

$$\frac{\partial J}{\partial U} = 0 \Rightarrow -f^T + H U^* = 0 \quad \boxed{U^* = H^{-1} f^T}$$

But in control engineering we always do $(y_{ref,h} - C_H A_H x_k)$ and not $(C_H A_H x_k - y_{ref,h})$

Therefore $\boxed{f = (y_{ref,h} - C_H A_H x_k)^T \cdot Q_H \cdot (C_H \cdot B_H)} \quad \boxed{H = (C_H B_H)^T \cdot Q_H \cdot (C_H \cdot B_H) + R_H}$

$\Rightarrow \boxed{U^* = -H^{-1} f^T}$ Ans

$$[H] \rightarrow 2N \times 2N$$

$$[f] \rightarrow \underbrace{(y_{ref,h} - C_H A_H x_k)^T}_{(2N \times 1)^T = 1 \times 2N} \cdot \underbrace{Q_H \cdot C_H \cdot B_H}_{2N \times 2N}$$

$$[f] \rightarrow 1 \times 2N$$

$$[f^T] \rightarrow 2N \times 1$$

$$[H^{-1}] \rightarrow 2N \times 2N$$

$$\begin{aligned} [H^{-1} f^T] &\rightarrow 2N \times 1 \\ [U^*] &\rightarrow 2N \times 1 \end{aligned}$$

Dimensionally
satisfied!!